Phi_Semantics/PhiSem_Machine_Integer.thy
@@ -234,6 +234,8 @@ lemma [\<phi>reason 800 for \<open>_ \<Ztypecolon> \<nat>(_) \<i>\<m>\<p>\<l>\<i
 \<Longrightarrow> x \<Ztypecolon> \<nat>('b) \<i>\<m>\<p>\<l>\<i>\<e>\<s> y \<Ztypecolon> \<nat>\<^sup>r('b) \<a>\<n>\<d> x < 2 ^ LENGTH('b)\<close>
   \<medium_left_bracket> destruct\<phi> _ \<medium_right_bracket>.
 
+declare [[\<phi>trace_reasoning = 2]]
+
 lemma [
   \<phi>reason 800 for \<open>_ \<Ztypecolon> \<nat>(_) \<i>\<m>\<p>\<l>\<i>\<e>\<s> _ \<a>\<n>\<d> _ @action to (\<phi>RoundedNat _)\<close>,
   \<phi>inhabitance_rule
