Phi_System/PhiSem_Formalization_Tools'.thy
@@ -380,7 +380,7 @@ lemma [THEN SE_clean_waste', \<phi>reason 1211]:
 lemma ToSA_by_structural_extraction:
   " Structure_Info U Q
 \<Longrightarrow> \<s>\<i>\<m>\<p>\<l>\<i>\<f>\<y> Q' : Q
-\<Longrightarrow> (Q' \<Longrightarrow> \<r>CALL Try Any (Structural_Extract (y \<Ztypecolon> \<phi> U) R1 (x \<Ztypecolon> \<phi> T) W P2))
+\<Longrightarrow> (<premise> Q' \<Longrightarrow> \<r>CALL Try Any (Structural_Extract (y \<Ztypecolon> \<phi> U) R1 (x \<Ztypecolon> \<phi> T) W P2))
 \<Longrightarrow> A \<i>\<m>\<p>\<l>\<i>\<e>\<s> R2 \<heavy_comma> \<blangle> W \<brangle> \<a>\<n>\<d> P1
 \<Longrightarrow> A \<heavy_comma> y \<Ztypecolon> \<phi> U \<i>\<m>\<p>\<l>\<i>\<e>\<s> R2\<heavy_comma> R1\<heavy_comma> \<blangle> x \<Ztypecolon> \<phi> T \<brangle> \<a>\<n>\<d> P1 \<and> P2"
   unfolding Premise_def FOCUS_TAG_def Structural_Extract_def Simplify_def Try_def \<r>Call_def
