Phi_System/Phi_BI.thy
@@ -175,8 +175,8 @@ lemma SubtyI[intro]: "Inhabited A \<Longrightarrow> A \<subseteq> B \<Longrighta
 
 lemma implies_trans:
   "A \<i>\<m>\<p>\<l>\<i>\<e>\<s> B \<a>\<n>\<d> P
-    \<Longrightarrow> (P \<Longrightarrow> B \<i>\<m>\<p>\<l>\<i>\<e>\<s> C \<a>\<n>\<d> Q)
-    \<Longrightarrow> A \<i>\<m>\<p>\<l>\<i>\<e>\<s> C \<a>\<n>\<d> P \<and> Q"
+\<Longrightarrow> (P \<Longrightarrow> B \<i>\<m>\<p>\<l>\<i>\<e>\<s> C \<a>\<n>\<d> Q)
+\<Longrightarrow> A \<i>\<m>\<p>\<l>\<i>\<e>\<s> C \<a>\<n>\<d> P \<and> Q"
   unfolding Imply_def by auto
 
 lemma implies_weaken:
