Phi_System/Phi_Types.thy
@@ -160,7 +160,7 @@ definition \<phi>Composition :: \<open>('v,'a) \<phi> \<Rightarrow> ('a,'b) \<ph
    
 lemma [\<phi>reason 1200]:
   \<open>x \<Ztypecolon> T \<Zcomp> U \<i>\<m>\<p>\<l>\<i>\<e>\<s> y \<Ztypecolon> T \<s>\<u>\<b>\<j> y. y \<in> (x \<Ztypecolon> U) @action to RAW\<close>
-  \<medium_left_bracket> destruct\<phi> _ thm useful  \<medium_right_bracket> .
+  \<medium_left_bracket> destruct\<phi> _ \<medium_right_bracket> .
 
 lemma [\<phi>reason 1200]:
   \<open> y \<Ztypecolon> Identity \<i>\<m>\<p>\<l>\<i>\<e>\<s> x \<Ztypecolon> U \<a>\<n>\<d> P
